theories/ThunksStep.v
@@ -16,6 +16,7 @@ Context `{inG Σ (authR max_natUR)}.                   (* γpaid *)
 
 Implicit Type p : na_inv_pool_name.
 Implicit Type N : namespace.
+Implicit Type E F : coPset.
 Implicit Type t : loc.
 Implicit Type n : nat.
 Implicit Type R : iProp.
@@ -42,84 +43,98 @@ Definition ThunkStepInv t γpaid nc R φ ψ : iProp :=
       )
 .
 
-Definition ThunkStep p N t n R ψ : iProp :=
+Definition ThunkStep p F t n R ψ : iProp :=
 
-  ∃ γpaid nc1 nc2 φ,
-      Thunk p (N .@ false) t nc1 R φ
-    ∗ na_inv p (N .@ true) (ThunkStepInv t γpaid nc2 R φ ψ)
+  ∃ γpaid nc1 nc2 φ F1 N,
+      ⌜ F1 ∪ ↑N ⊆ F ⌝
+    ∗ ⌜ F1 ∩ ↑N = ∅ ⌝
+    ∗ Thunk p F1 t nc1 R φ
+    ∗ na_inv p N (ThunkStepInv t γpaid nc2 R φ ψ)
     ∗ own γpaid (◯ MaxNat (nc1 + nc2 - n))
 
 .
 
 (* -------------------------------------------------------------------------- *)
 
-Global Instance thunkstep_persistent p N t n R ψ :
-  Persistent (ThunkStep p N t n R ψ).
+(* Local tactics, for clarity. *)
+
+Local Ltac destruct_thunk :=
+  iDestruct "Hthunk"
+    as (γpaid nc1 nc2 φ F1 N) "(%HuF & %HnF & Hthunk & Hinv & Hγpaid◯)".
+
+Local Ltac open_invariant :=
+  iDestruct (na_inv_acc with "Hinv Hp") as ">(Hstepinv & Hp & Hclose)";
+    [ set_solver | set_solver |].
+
+Local Ltac pure_conjunct :=
+  iSplitR; [ iPureIntro; eauto |].
+
+(* -------------------------------------------------------------------------- *)
+
+Global Instance thunkstep_persistent p F t n R ψ :
+  Persistent (ThunkStep p F t n R ψ).
 Proof.
   exact _.
 Qed.
 
 (* -------------------------------------------------------------------------- *)
 
-Lemma thunkstep_weakening p N t n1 n2 R ψ :
+Lemma thunkstep_weakening p F t n1 n2 R ψ :
   n1 ≤ n2 →
-  ThunkStep p N t n1 R ψ -∗
-  ThunkStep p N t n2 R ψ.
+  ThunkStep p F t n1 R ψ -∗
+  ThunkStep p F t n2 R ψ.
 Proof.
   iIntros (?) "Hthunk".
-  iDestruct "Hthunk" as (γpaid nc1 nc2 φ) "(? & ? & Hγpaid◯)".
-  iExists γpaid, nc1, nc2, φ. iFrame.
+  destruct_thunk.
+  iExists γpaid, nc1, nc2, φ, F1, N.
+  repeat pure_conjunct.
+  iFrame.
   iDestruct (own_auth_max_nat_weaken with "Hγpaid◯") as "$".
   lia.
 Qed.
 
 (* -------------------------------------------------------------------------- *)
 
-Lemma thunkstep_consequence E p N t n1 n2 n R φ ψ :
+Lemma thunkstep_consequence E p F1 N F t n1 n2 n R φ ψ :
+  F1 ∪ ↑N ⊆ F →
+  F1 ∩ ↑N = ∅ →
   TC 0 -∗ (* TODO get rid of this? *)
-  Thunk p (N .@ false) t n1 R φ -∗ (* TODO namespace trouble? *)
-  (∀ v, R -∗ TC n2 -∗ □ φ v ={⊤}=∗ R ∗ □ ψ v) -∗
-  ⌜ n1 + n2 ≤ n ⌝ ={E}=∗
-  ThunkStep p N t n R ψ.
+  Thunk p F1 t n1 R φ -∗
+  (∀ v, R -∗ TC n2 -∗ □ φ v ={⊤}=∗ R ∗ □ ψ v) ={E}=∗
+  ThunkStep p F t (n1 + n2) R ψ.
 Proof.
-  iIntros "Hcredits #Hthunk Hupdate %Hleq".
+  iIntros (? ?) "Hcredits #Hthunk Hupdate".
   (* Allocate the ghost cell γpaid. *)
   iMod (auth_max_nat_alloc 0) as (γpaid) "[Hγpaid● Hγpaid◯]".
-  iExists γpaid, n1, n2, φ.
-  rewrite (_ : n1 + n2 - n = 0); [| lia].
-  iFrame "Hthunk".
-  iFrame "Hγpaid◯".
+  iExists γpaid, n1, n2, φ, F1, N.
+  rewrite Nat.sub_diag.
+  repeat pure_conjunct.
+  iFrame "Hthunk Hγpaid◯".
   (* Allocate the invariant. *)
   iApply na_inv_alloc.
   iNext.
   (* The number of available credits is initially zero. *)
-  iExists 0.
-  iFrame "Hγpaid●".
-  (* The left-hand disjunct initially holds. *)
-  iLeft.
-  iFrame "Hcredits Hupdate".
+  iExists 0. eauto with iFrame.
 Qed.
 
 (* -------------------------------------------------------------------------- *)
 
 (* A public lemma: the specification of [force]. *)
 
-Lemma thunkstep_force_spec p N F t R ψ :
-  ↑N ⊆ F →
+Lemma thunkstep_force_spec p F F' t R ψ :
+  F ⊆ F' →
   TC_invariant -∗
-  {{{ TC 11 ∗ ThunkStep p N t 0 R ψ ∗ na_own p F ∗ R }}}
+  {{{ TC 11 ∗ ThunkStep p F t 0 R ψ ∗ ThunkToken p F' ∗ R }}}
     «force #t»
-  {{{ v, RET «v» ; □ ψ v ∗ ThunkVal t v ∗ na_own p F ∗ R }}}.
+  {{{ v, RET «v» ; □ ψ v ∗ ThunkVal t v ∗ ThunkToken p F' ∗ R }}}.
 Proof.
   intros ?.
   iIntros "#Htickinv" (Φ) "!> (Hcredits & #Hthunk & Hp & HR) Post".
-  iDestruct "Hthunk" as (γpaid nc1 nc2 φ) "#(Hthunk & Hinv & Hγpaid◯)".
+  destruct_thunk.
   rewrite Nat.sub_0_r. (* nc - 0 = nc *)
 
   (* Open the invariant. *)
-  iDestruct (na_inv_acc with "Hinv Hp")
-    as ">(Hstepinv & Hp & Hclose)";
-    [done|eauto with ndisj|]. (* side conditions about masks *)
+  open_invariant.
 
   (* Perform a case analysis. *)
   iDestruct "Hstepinv" as (ac) "(>Hγpaid● & [ Hstepinv | Hstepinv ])".
@@ -137,7 +152,7 @@ Proof.
     iApply wp_fupd.
     (* Force the underlying thunk. *)
     iApply (thunk_pay_force with "Htickinv [$Hnc1 $Hthunk $Hp $HR]").
-    { eauto with ndisj. }
+    { set_solver. }
     (* This has consumed at least one time step. (This is fortunate.) *)
     iNext.
     iIntros (v) "(#Hv & #Hval & Hp & HR)".
@@ -154,7 +169,7 @@ Proof.
     (* Done. *)
     iModIntro.
     iApply "Post".
-    iFrame "Hv Hval Hp HR".
+    eauto with iFrame.
   }
 
   (* Case: the ghost update has been used already. *)
@@ -167,7 +182,7 @@ Proof.
        The result must be [v]. We do not obtain [□ φ v], but
        we do not need it. *)
     iApply (thunk_force_forced_weak with "Htickinv [$Hcredits $Hthunk $Hval $Hp $HR]").
-    { eauto with ndisj. }
+    { set_solver. }
     iNext.
     iDestruct "Hv" as "#Hv".
     iIntros "(Hp & HR)".
@@ -178,20 +193,20 @@ Proof.
     (* Done. *)
     iApply "Post".
     iModIntro.
-    iFrame "Hv Hval Hp HR".
+    eauto with iFrame.
   }
 Qed.
 
-Lemma thunkstep_force_forced_weak p N t n R ψ v F :
-  ↑N ⊆ F →
+Lemma thunkstep_force_forced_weak p F t n R ψ v F' :
+  F ⊆ F' →
   TC_invariant -∗
-  {{{ TC 11 ∗ ThunkStep p N t n R ψ ∗ ThunkVal t v ∗ na_own p F ∗ R }}}
+  {{{ TC 11 ∗ ThunkStep p F t n R ψ ∗ ThunkVal t v ∗ ThunkToken p F' ∗ R }}}
     «force #t»
-  {{{ RET «v» ; na_own p F ∗ R }}}.
+  {{{ RET «v» ; ThunkToken p F' ∗ R }}}.
 Proof.
   intros ?.
   iIntros "#Htickinv" (Φ) "!> (Hcredits & #Hthunk & #Hval & Hp & HR) Post".
-  iDestruct "Hthunk" as (γpaid nc1 nc2 φ) "#(Hthunk & _ & _)".
+  destruct_thunk. iClear "Hinv Hγpaid◯".
 
   (* Remarkably, we do not even need to open the invariant. *)
 
@@ -201,27 +216,26 @@ Proof.
 
   iApply (thunk_force_forced_weak
     with "Htickinv [$Hcredits $Hthunk $Hval $Hp $HR]");
-    [ eauto with ndisj |].
+    [ set_solver |].
 
   (* Done. *)
   eauto.
 
 Qed.
 
-Lemma thunkstep_pay p N F E n k t R ψ :
-  ↑N ⊆ F →
-  ↑N ⊆ E →
-  na_own p F -∗ ThunkStep p N t n R ψ -∗
+Lemma thunkstep_pay p F F' E n k t R ψ :
+  F ⊆ F' →
+  F ⊆ E →
+  ThunkToken p F' -∗ ThunkStep p F t n R ψ -∗
   TC k ={E}=∗
-  na_own p F  ∗ ThunkStep p N t (n-k) R ψ.
+  ThunkToken p F'  ∗ ThunkStep p F t (n-k) R ψ.
 Proof.
   iIntros (? ?) "Hp #Hthunk Hk".
-  iDestruct "Hthunk" as (γpaid nc1 nc2 φ) "#(Hthunk & Hinv & Hγpaid◯)".
+  destruct_thunk.
 
   (* Open the invariant. *)
-  iDestruct (na_inv_acc with "Hinv Hp") as ">(Hstep & Hp & Hclose)";
-    [ eauto with ndisj | eauto with ndisj |].
-  iDestruct "Hstep" as (ac) "(>Hγpaid● & Hstep)".
+  open_invariant.
+  iDestruct "Hstepinv" as (ac) "(>Hγpaid● & Hstep)".
 
   (* Increment the ghost payment record from [ac] to [ac + k]. This is
      done in both branches of the case analysis (which follows). *)
@@ -241,7 +255,8 @@ Proof.
     iMod ("Hclose" with "[-Hγpaid◯]") as "$".
     { iFrame "Hp". iNext. iExists (ac+k). auto with iFrame. }
     iModIntro.
-    iExists γpaid, nc1, nc2, φ. iFrame "Hthunk Hinv".
+    iExists γpaid, nc1, nc2, φ, F1, N. iFrame "Hthunk Hinv".
+    repeat pure_conjunct.
     (* Our updated fragmentary view of the ghost cell γpaid
        allows us to produce an updated [Thunk] assertion. *)
     iApply (own_auth_max_nat_weaken with "[$]").
@@ -257,7 +272,8 @@ Proof.
     iMod ("Hclose" with "[-Hγpaid◯]") as "$".
     { iFrame "Hp". iNext. iExists (ac+k). auto with iFrame. }
     iModIntro.
-    iExists γpaid, nc1, nc2, φ. iFrame "Hthunk Hinv".
+    iExists γpaid, nc1, nc2, φ, F1, N. iFrame "Hthunk Hinv".
+    repeat pure_conjunct.
     iApply (own_auth_max_nat_weaken with "[$]").
     lia.
   }
